Algorithm.dfy
@@ -25,60 +25,26 @@ module Algorithm {
       this.s := s;
       this.t := t;
       this.c := c;
-
       new;
+
+      f := seq(V, _ => seq(V, _ => 0));
+      e := seq(V, _ => 0); // initialize excess to 0, will be overwritten in the loop
 
       buckets := seq(2 * V, _ => {});
       max_height := 0;
 
-      for v := 0 to V
-        // capacityConstraint
-        invariant forall i: Node, j: Node | i < v :: f[i][j] <= c[i][j]
-
-        // invariant to prove skewSymmetryConstraint
-        invariant forall i: Node, j: Node | i < v :: f[i][j] == 0
-
-        // invariant so Dafny does not forget
-        invariant forall h: nat | 0 <= h < 2 * V :: |buckets[h]| == 0
-      {
-        for w := 0 to V
-          // capacity constraint
-          invariant forall i: Node, j: Node | i < v :: f[i][j] <= c[i][j]
-          invariant forall j: Node | j < w :: f[v][j] <= c[v][j]
-
-          // invariant to prove skewSymmetryConstraint
-          invariant forall i: Node, j: Node | i < v :: f[i][j] == 0
-          invariant forall j: Node | j < w :: f[v][j] == 0
-
-          // invariant so Dafny does not forget
-          invariant forall h: nat | 0 <= h < 2 * V :: |buckets[h]| == 0
-        {
-          f := f[v := f[v][w := 0]];
-        }
-      }
-      assert ValidCapacityConstraint(c, f);
-
-      assert forall i: Node, j: Node :: f[i][j] == 0;
-      assert ValidSkewSymmetryConstraint(f);
-
-      // assert by lemma
-      assert ValidNonnegativityConstraint(s, f) by {
-        forall v: Node {:trigger SumTotalFlowToNode(f, v, V - 1)} {
-          Lemma_ZeroFlowEqualsZeroSumFlowInOfNode(f, v, V - 1);
-        }
-      }
-
       // needed to prove matching invariant on entry
+      // assert forall i: Node {:trigger SumTotalFlowToNode(f, i, V - 1)} | i != s :: SumTotalFlowToNode(f, i, V - 1) == 0 by {
+      //   forall v: Node {:trigger SumTotalFlowToNode(f, v, V - 1)} {
+      //     Lemma_ZeroFlowEqualsZeroSumFlowInOfNode(f, v, V - 1);
+      //   }
+      // }
       assert forall i: Node {:trigger SumTotalFlowToNode(f, i, V - 1)} | i != s :: SumTotalFlowToNode(f, i, V - 1) == 0 by {
         forall v: Node {:trigger SumTotalFlowToNode(f, v, V - 1)} {
           Lemma_ZeroFlowEqualsZeroSumFlowInOfNode(f, v, V - 1);
         }
       }
-
-      // for proving ValidBuckets(s, t, e, d, max_height, buckets) holds on entry
-      assert forall h: nat | 0 <= h < 2 * V :: |buckets[h]| == 0;
-      e := seq(V, _ => 0); // initialize excess to 0, will be overwritten in the loop
-      assert forall v: Node :: e[v] == 0;
+      assert ValidNonnegativityConstraint(s, f);
 
       for v := 0 to V
         invariant ValidCapacityConstraint(c, f)
@@ -91,14 +57,15 @@ module Algorithm {
         invariant forall i: Node | i != s && i < v :: e[i] == SumTotalFlowToNode(f, i, V - 1)
 
         // invariant needed to prove f_old[s][i] == 0
-        // which is needed for the call to Lemma_FlowSumAfterPush(f_old, f, s, v, delta, V - 1)
+        // which is needed for the call to Lemma_FlowSumAfterPush
         invariant forall i: Node | i >= v :: f[s][i] == 0
 
-        // for provid ValidLabeling(s, t, c, f, d)
+        // for proving ValidLabeling(s, t, c, f, d)
         invariant forall i: Node | i != s && i < v :: d[i] == 0
         invariant forall i: Node | i != s && i < v :: ResidualCapacity(c, f, s, i) == 0
 
         // for proving ValidBuckets(s, t, e, d, max_height, buckets)
+        invariant max_height == 0
         invariant ValidBuckets(s, t, e, d, max_height, buckets)
         invariant forall h: nat, i: Node | 0 <= h < 2 * V && i >= v :: i !in buckets[h]
       {
@@ -115,25 +82,18 @@ module Algorithm {
         Lemma_FlowSumAfterPush(f_old, f, s, v, delta, V - 1);
         assert ValidNonnegativityConstraint(s, f);
 
-        assert ResidualCapacity(c, f, s, v) == 0;
-        // assert that residual capacity of all nodes before v is unchanged
+        // assert that residual capacity of s to all nodes before v is unchanged
+        // needed to prove invariant ResidualCapacity(c, f, s, i) == 0 for all i != s && i < v
         assert forall i: Node | i != s && i < v :: ResidualCapacity(c, f, s, i) == ResidualCapacity(c, f_old, s, i);
-        // which means it is also 0 (combining previous two assertions)
-        assert forall i: Node | i != s && i < v + 1 :: ResidualCapacity(c, f, s, i) == 0;
+        // and assert that residual capacity of s to v is 0
+        assert ResidualCapacity(c, f, s, v) == 0;
 
-        ghost var d_old := d;
         d := d[v := 0];
 
-        assert SumTotalFlowToNode(f, v, V - 1) == delta;
-        ghost var e_old := e;
         e := e[v := delta];
 
-        ghost var buckets_old := buckets;
         if (e[v] > 0 && v != t) {
-          buckets := buckets[d[v] := buckets[d[v]] + {v}];
-          if (d[v] > max_height) {
-            max_height := d[v];
-          }
+          buckets := buckets[0 := buckets[0] + {v}];
         }
       }
       d := d[s := V];
@@ -168,10 +128,11 @@ module Algorithm {
       requires ResidualCapacity(c, f, v, w) > 0 // There must be residual capacity to move
       requires d[v] == d[w] + 1                 // Water must flow exactly one step downhill
 
-      // postconditions
+      // Postconditions for correctness
       ensures ValidWithPreflow()
-      ensures max_height >= 0
       ensures max_height == old(max_height)
+
+      // Postconditions for termination
       ensures e[v] < old(e[v])
       ensures d == old(d)
       ensures buckets[d[v]] == old(buckets)[d[v]] || buckets[d[v]] == old(buckets)[d[v]] - {v}
@@ -222,9 +183,11 @@ module Algorithm {
       // v cannot be relabeled if it has a downhill neighbor
       requires forall w: Node | (ResidualCapacity(c, f, v, w) > 0) :: d[v] <= d[w]
 
-      // Postconditions
+      // Postconditions for correctness
       ensures ValidWithPreflow()
-      ensures max_height >= 0
+      ensures max_height >= old(max_height)
+
+      // Postconditions for termination
       ensures e == old(e)
       ensures d[v] > old(d[v])
       ensures forall i: Node | i != v :: d[i] == old(d)[i]
@@ -306,7 +269,7 @@ module Algorithm {
 
       ensures ValidWithPreflow()
       ensures e[v] == 0
-      ensures max_height >= 0
+      ensures max_height >= old(max_height)
 
       ensures LabelingMetric(d, V) <= LabelingMetric(old(d), V)
       ensures d != old(d) ==> LabelingMetric(d, V) < LabelingMetric(old(d), V)
@@ -320,7 +283,7 @@ module Algorithm {
 
       while (e[v] > 0)
         invariant ValidWithPreflow()
-        invariant max_height >= 0
+        invariant max_height >= old(max_height)
 
         invariant LabelingMetric(d, V) <= LabelingMetric(start_d, V)
         invariant d != start_d ==> LabelingMetric(d, V) < LabelingMetric(start_d, V)
@@ -349,7 +312,9 @@ module Algorithm {
 
     method CalculateMaxFlow()
       requires ValidWithPreflow()
+
       ensures ValidWithFlow()
+      ensures !SimpleResidualPathExists(c, f, s, t)
 
       modifies this
     {
@@ -372,6 +337,7 @@ module Algorithm {
       }
 
       // show dafny that ValidFLowConservationConstraint holds
+      assert max_height == -1;
       assert forall v: Node | v != s && v != t :: e[v] == 0;
       assert forall v: Node {:trigger SumTotalFlowToNode(f, v, V - 1)} | (v != s && v != t) :: SumTotalFlowToNode(f, v, V - 1) == e[v];
       assert ValidFlowConservationConstraint(s, t, f);
@@ -379,10 +345,8 @@ module Algorithm {
       // assert that we have valid variables and a valid flow
       assert ValidWithFlow();
 
-      // 2. Prove the Flow is Maximal!
+      // show dafny that there is no residual path from s to t (which means the flow is maximal)
       Lemma_NoResidualPathFromSToT(s, t, c, f, d);
-      assert !(exists p: Path :: IsSimpleResidualPath(c, f, p) && p[0] == s && p[|p|-1] == t);
-      assert ValidFlow(s, t, c, f);
     }
   }
 }
